src/Transforms/Shallow.dfy
@@ -1,29 +1,71 @@
+include "../AST/Entities.dfy"
 include "../AST/Syntax.dfy"
 include "../AST/Predicates.dfy"
 include "Generic.dfy"
 
 module Bootstrap.Transforms.Shallow {
   import opened Utils.Lib
+  import opened Utils.Lib.Datatypes
+  import opened AST.Entities
   import opened AST.Syntax
   import opened AST.Predicates
   import opened Generic
 
-  function method {:opaque} Map_Method(m: Method, tr: ExprTransformer) : (m': Method)
-    requires Shallow.All_Method(m, tr.f.requires)
-    ensures Shallow.All_Method(m', tr.post) // FIXME Deep
+  function method Map_Option<S,T>(f: S ~> T, o: Option<S>): Option<T>
+    reads f.reads
+    requires o.Some? ==> f.requires(o.value)
   {
-    match m {
-      case Method(CompileName, methodBody) =>
-        Method (CompileName, tr.f(methodBody))
+    match o {
+      case None => None
+      case Some(x) => Some(f(x))
     }
   }
+
+  function method {:opaque} Map_Callable(c: Callable, tr: ExprTransformer) : (c': Callable)
+    requires Shallow.All_Callable(c, tr.f.requires)
+    ensures Shallow.All_Callable(c', tr.post) // FIXME Deep
+  {
+    var req' := Seq.Map(tr.f, c.req);
+    var ens' := Seq.Map(tr.f, c.ens);
+    var body' := Map_Option(tr.f, c.body);
+    match c {
+      case Constructor(_, _, _) => Constructor(req', ens', body')
+      case Function(_, _, _) => Function(req', ens', body')
+      case Method(_, _, _) => Method(req', ens', body')
+    }
+  }
+
+  function method {:opaque} Map_Entity(e: Entity, tr: ExprTransformer) : (e': Entity)
+    requires Shallow.All_Entity(e, tr.f.requires)
+    ensures Shallow.All_Entity(e', tr.post)
+    ensures e'.kind == e.kind
+    ensures e'.ei.name == e.ei.name
+    ensures e'.ei.members == e.ei.members
+  {
+    match e {
+      case Definition(ei, d) =>
+        if d.Callable? then
+          Definition(ei, Callable(Map_Callable(d.ci, tr)))
+        else e
+      // TODO: add fields once they contain expressions
+      case _ => e
+    }
+  }
+
+  function method Map_EntityTransformer(tr: ExprTransformer): (Entity --> Entity) {
+    e requires Shallow.All_Entity(e, tr.f.requires) => Map_Entity(e, tr)
+  }
+
+  // TODO: prove!
+  lemma Map_EntityIsEntityTransformer(tr: ExprTransformer)
+    ensures EntityTransformer?(Map_EntityTransformer(tr))
 
   function method {:opaque} Map_Program(p: Program, tr: ExprTransformer) : (p': Program)
     requires Shallow.All_Program(p, tr.f.requires)
     ensures Shallow.All_Program(p', tr.post)
   {
-    match p {
-      case Program(mainMethod) => Program(Map_Method(mainMethod, tr))
-    }
+    Map_EntityIsEntityTransformer(tr);
+    var reg' := p.registry.Map(Map_EntityTransformer(tr));
+    Program(reg', defaultModule := p.defaultModule, mainMethod := p.mainMethod)
   }
 }
